Reduce cheats in steph_fill_step to ones about ffi encoding
Specifically, now just need to know preamble_env does plausible things,
and that encode_output is injective.

The other cheat about computeEvents ignoring policies also remains.

botworld_propsScript.sml
@@ -1291,6 +1291,340 @@ val FST_if_focal = Q.store_thm("FST_if_focal[simp]",
 
 open match_goal
 
+(* TODO: move *)
+
+open terminationTheory
+
+val ffi_state_rel_def = Define`
+  ffi_state_rel oracle R s1 s2 ⇔
+    s1.oracle = oracle ∧ s2.oracle = oracle ∧
+    R s1.ffi_state s2.ffi_state ∧
+    s2 = s1 with ffi_state := s2.ffi_state`;
+
+val ffi_rel_def = Define`
+  ffi_rel oracle R s1 s2 ⇔
+    ffi_state_rel oracle R s1.ffi s2.ffi ∧
+    s2 = s1 with ffi := s2.ffi`;
+
+val ffi_rel_dec_clock = Q.store_thm("ffi_rel_dec_clock",
+  `ffi_rel or R s1 s2 ⇒
+   ffi_rel or R (dec_clock s1) (dec_clock s2)`,
+  EVAL_TAC \\ rw[semanticPrimitivesTheory.state_component_equality]);
+
+val ffi_rel_same_clock = Q.store_thm("ffi_rel_same_clock",
+  `ffi_rel or R s1 s2 ⇒ s1.clock = s2.clock`,
+  EVAL_TAC \\ rw[semanticPrimitivesTheory.state_component_equality]);
+
+val ffi_rel_same_refs = Q.store_thm("ffi_rel_same_refs",
+  `ffi_rel or R s1 s2 ⇒ s1.refs = s2.refs`,
+  EVAL_TAC \\ rw[semanticPrimitivesTheory.state_component_equality]);
+
+val ffi_rel_same_defined_mods = Q.store_thm("ffi_rel_same_defined_mods",
+  `ffi_rel or R s1 s2 ⇒ s1.defined_mods = s2.defined_mods`,
+  EVAL_TAC \\ rw[semanticPrimitivesTheory.state_component_equality]);
+
+val ffi_rel_same_defined_types = Q.store_thm("ffi_rel_same_defined_types",
+  `ffi_rel or R s1 s2 ⇒ s1.defined_types = s2.defined_types`,
+  EVAL_TAC \\ rw[semanticPrimitivesTheory.state_component_equality]);
+
+fun extends_tac (tac:tactic) ((g as (asl,w)):goal) =
+  let
+    val asms1 = HOLset.fromList Term.compare asl
+    val (gs,v) = tac g
+    fun extends asl =
+      let
+        val asms2 = HOLset.fromList Term.compare asl
+      in not (HOLset.isEmpty (HOLset.difference(asms2,asms1))) end
+  in
+    (assert(List.all (extends o #1)) gs,v)
+  end
+
+val call_FFI_invariant_def = Define`
+  call_FFI_invariant oracle R ⇔
+  ∀ffi ffi'.
+    ffi.oracle = oracle ∧
+    ffi' = ffi with ffi_state := ffi'.ffi_state ∧
+    R ffi.ffi_state ffi'.ffi_state ⇒
+    ∀i ws.
+      let (ffj,vs) = call_FFI ffi i ws in
+      let (ffj',vs') = call_FFI ffi' i ws in
+        R ffj.ffi_state ffj'.ffi_state
+        ∧ ffj' = ffj with ffi_state := ffj'.ffi_state
+        ∧ vs = vs'`;
+
+val do_app_ffi_extensional = Q.store_thm("do_app_ffi_extensional",
+  `call_FFI_invariant oracle R ∧
+   ffi_state_rel oracle R ffi1 ffi2 ⇒
+   OPTION_REL
+    (λ((refs1,ffi1),res1) ((refs2,ffi2),res2).
+       refs1 = refs2 ∧ res1 = res2 ∧
+       ffi2 = ffi1 with ffi_state := ffi2.ffi_state ∧
+       ffi1.oracle = oracle ∧ ffi2.oracle = oracle ∧
+       R ffi1.ffi_state ffi2.ffi_state)
+    (do_app (refs,ffi1) op es)
+    (do_app (refs,ffi2) op es)`,
+  (match1_tac(mg.acb`o_ : 'a option`,(fn(a,t)=>extends_tac(Cases_on`^(t("o"))` \\fs[]\\rveq))))
+  \\ fs[OPTREL_def]
+  \\ rpt (match1_tac(mg.acb`o_ : 'a # 'b`,(fn(a,t)=>extends_tac(Cases_on`^(t("o"))` \\fs[]\\rveq))))
+  >- (
+    reverse(Cases_on`op`)\\fs[semanticPrimitivesTheory.do_app_def]
+    \\ every_case_tac \\ fs[UNCURRY]
+    \\ spose_not_then strip_assume_tac
+    \\ fs[call_FFI_invariant_def,ffi_state_rel_def]
+    \\ match_tac([mg.a"1"`_`,mg.a"2"`_`,mg.a"3"`_`], fn(a,t)=>
+                 first_x_assum(drule_thm(LIST_CONJ (map a ["1","2","3"]))))
+    \\ simp[]
+    \\ qmatch_assum_rename_tac`call_FFI _ i ws = _`
+    \\ map_every qexists_tac[`i`,`ws`]
+    \\ simp[]
+    \\ spose_not_then strip_assume_tac
+    \\ fs[] )
+  \\ rw[ffi_state_rel_def,ffiTheory.ffi_state_component_equality]
+  \\ fs[evalPropsTheory.do_app_cases,semanticPrimitivesTheory.do_app_def] \\ rw[]
+  \\ every_case_tac \\ fs[]
+  \\ spose_not_then strip_assume_tac
+  \\ fs[call_FFI_invariant_def,ffiTheory.ffi_state_component_equality,GSYM CONJ_ASSOC]
+  \\ match_tac([mg.a"1"`_`,mg.a"2"`_`,mg.a"3"`_`,mg.a"4"`_`], fn(a,t)=>
+               first_x_assum(drule_thm(LIST_CONJ [REFL(rhs(concl(a"1"))),a"1",a"2",a"3",a"4"])))
+  \\ simp[]
+  \\ qmatch_assum_rename_tac`call_FFI _ i ws = _`
+  \\ map_every qexists_tac[`i`,`ws`]
+  \\ simp[]
+  \\ spose_not_then strip_assume_tac
+  \\ fs[]
+  \\ fs[ffiTheory.ffi_state_component_equality]
+  \\ rveq \\ fs[]
+  \\ fs[ffiTheory.call_FFI_def]
+  \\ every_case_tac \\ fs[] \\ rveq \\ fs[]);
+
+val evaluate_ffi_extensional = Q.store_thm("evaluate_ffi_extensional",
+  `call_FFI_invariant oracle R ⇒
+   (∀st env es st' res res' st2 st2'.
+      ffi_rel oracle R st st' ∧
+      evaluate st env es = (st2,res) ∧
+      evaluate st' env es = (st2',res')
+      ⇒ res = res' ∧ ffi_rel oracle R st2 st2') ∧
+   (∀st env v pes err_v st' res res' st2 st2'.
+       ffi_rel oracle R st st' ∧
+       evaluate_match st env v pes err_v = (st2,res) ∧
+       evaluate_match st' env v pes err_v = (st2',res')
+       ⇒ res = res' ∧ ffi_rel oracle R st2 st2')`,
+  strip_tac
+  \\ ho_match_mp_tac evaluate_ind
+  \\ rpt conj_tac
+  \\ rpt gen_tac \\ simp[evaluate_def] \\ strip_tac
+  \\ rveq \\ rpt gen_tac \\ fs[] \\ strip_tac
+  \\ TRY (
+    every_case_tac
+  \\ rpt (qpat_assum`_ ∧ _`strip_assume_tac) \\ rveq
+  \\ fs[] \\ rfs[] \\ rveq
+  \\ imp_res_tac ffi_rel_same_refs \\ fs[]
+  \\ first_x_assum drule \\ fs[]
+  \\ rpt( strip_tac \\ rveq)
+  \\ spose_not_then strip_assume_tac \\ fs[] \\ rveq
+  \\ first_x_assum drule \\ fs[])
+  (* App case *)
+  \\ every_case_tac
+  \\ rpt (qpat_assum`_ ∧ _`strip_assume_tac) \\ rveq
+  \\ fs[] \\ rfs[] \\ rveq
+  \\ imp_res_tac ffi_rel_same_refs \\ fs[]
+  \\ first_x_assum drule \\ fs[]
+  \\ rpt( strip_tac \\ rveq)
+  \\ spose_not_then strip_assume_tac \\ fs[] \\ rveq
+  \\ imp_res_tac ffi_rel_dec_clock
+  \\ imp_res_tac ffi_rel_same_clock \\ fs[]
+  \\ TRY(first_x_assum drule \\ fs[])
+  \\ imp_res_tac ffi_rel_same_refs \\ fs[]
+  \\ imp_res_tac do_app_ffi_extensional
+  \\ fs[ffi_rel_def,
+        semanticPrimitivesTheory.state_component_equality,
+        funBigStepTheory.dec_clock_def]
+  \\ match_tac(
+       [mg.a"h"`ffi_state_rel _ R ffi_ _`,
+        mg.bau`do_app (refs_,ffi_) op_ es_`
+       ],
+       fn(a,t)=>first_x_assum(drule_thm(a"h")) \\ simp[]
+                \\ map_every (exists_tac o t) ["refs","op","es"])
+  \\ simp[OPTREL_def]
+  \\ spose_not_then strip_assume_tac \\ fs[]
+  \\ rveq \\ fs[]
+  \\ fs[ffi_state_rel_def]);
+
+val encoded_ffi_def = Define`
+  encoded_ffi ffi1 ffi2 ⇔
+    encode_observation ffi1.bot_input =
+    encode_observation ffi2.bot_input ∧
+    encode_output ffi1.bot_output =
+    encode_output ffi2.bot_output`;
+
+val evaluate_decs_ffi_extensional = Q.store_thm("evaluate_decs_ffi_extensional",
+  `call_FFI_invariant oracle R ⇒
+   ∀mn st env decs st' res res' st2 st2'.
+   ffi_rel oracle R st st' ∧
+   evaluate_decs mn st env decs = (st2,res) ∧
+   evaluate_decs mn st' env decs = (st2',res')
+   ⇒
+   res = res' ∧ ffi_rel oracle R st2 st2'`,
+  strip_tac
+  \\ ho_match_mp_tac funBigStepTheory.evaluate_decs_ind
+  \\ rw[funBigStepTheory.evaluate_decs_def] \\ rw[]
+  \\ imp_res_tac ffi_rel_same_defined_types \\ fs[]
+  \\ every_case_tac \\ fs[] \\ rw[] \\ rfs[] \\ fs[]
+  \\ TRY (
+    first_x_assum drule \\ disch_then drule \\ rw[]
+    \\ first_x_assum drule \\ disch_then drule \\ rw[])
+  \\ imp_res_tac (CONJUNCT1 (UNDISCH evaluate_ffi_extensional)) \\ fs[]
+  \\ rveq \\ fs[]
+  \\ imp_res_tac ffi_rel_same_refs \\ fs[]
+  \\ fs[ffi_rel_def,semanticPrimitivesTheory.state_component_equality]);
+
+val evaluate_tops_ffi_extensional = Q.store_thm("evaluate_tops_ffi_extensional",
+  `call_FFI_invariant oracle R ⇒
+   ∀st env tops st' res res' st2 st2'.
+   ffi_rel oracle R st st' ∧
+   evaluate_tops st env tops = (st2,res) ∧
+   evaluate_tops st' env tops = (st2',res')
+   ⇒
+   res = res' ∧ ffi_rel oracle R st2 st2'`,
+  strip_tac
+  \\ ho_match_mp_tac funBigStepTheory.evaluate_tops_ind
+  \\ rw[funBigStepTheory.evaluate_tops_def] \\ rw[]
+  \\ imp_res_tac ffi_rel_same_defined_mods \\ fs[]
+  \\ every_case_tac \\ fs[] \\ rw[] \\ rfs[] \\ fs[]
+  \\ TRY (
+    first_x_assum drule \\ disch_then drule \\ rw[]
+    \\ first_x_assum drule \\ disch_then drule \\ rw[])
+  \\ imp_res_tac (UNDISCH evaluate_decs_ffi_extensional) \\ fs[]
+  \\ rveq \\ fs[]
+  \\ imp_res_tac ffi_rel_same_refs \\ fs[]
+  \\ fs[ffi_rel_def,semanticPrimitivesTheory.state_component_equality]);
+
+val evaluate_prog_ffi_extensional = Q.store_thm("evaluate_prog_ffi_extensional",
+  `call_FFI_invariant oracle R ⇒
+   ffi_rel oracle R st st' ∧
+   evaluate_prog st env prog = (st2,res) ∧
+   evaluate_prog st' env prog = (st2',res')
+   ⇒
+   res = res' ∧ ffi_rel oracle R st2 st2'`,
+  simp[funBigStepTheory.evaluate_prog_def]
+  \\ ntac 2 strip_tac
+  \\ imp_res_tac ffi_rel_same_defined_mods
+  \\ imp_res_tac ffi_rel_same_defined_types
+  \\ fs[]
+  \\ every_case_tac \\ fs[]
+  \\ metis_tac[evaluate_tops_ffi_extensional]);
+
+(* -- *)
+
+val botworld_call_FFI_invariant = Q.store_thm("botworld_call_FFI_invariant",
+  `call_FFI_invariant botworld_oracle encoded_ffi`,
+  rw[call_FFI_invariant_def,ffiTheory.call_FFI_def,encoded_ffi_def]
+  \\ pairarg_tac \\ fs[] \\ pairarg_tac \\ fs[]
+  \\ fs[ffiTheory.ffi_state_component_equality]
+  \\ rfs[]
+  \\ every_case_tac \\ fs[] \\ rveq \\ fs[]
+  \\ fs[botworld_serialiseTheory.botworld_oracle_def]
+  \\ every_case_tac
+  \\ fs[botworld_serialiseTheory.botworld_read_def,
+        botworld_serialiseTheory.botworld_write_def,
+        botworld_serialiseTheory.botworld_get_output_length_def,
+        botworld_serialiseTheory.botworld_get_input_length_def,
+        botworld_serialiseTheory.botworld_read_output_def]
+  \\ every_case_tac \\ fs[] \\ rfs[] \\ rveq \\ fs[]);
+
+val ffi_from_observation_with_memory = Q.store_thm("ffi_from_observation_with_memory",
+  `obs1 = FST (prepare x y) ∧ obs2 = FST (prepare x' y) ∧
+   x' = x with robotActions updated_by (MAP (if_focal nm (with_memory p ## I)))
+   ⇒
+   ffi_state_rel botworld_oracle encoded_ffi
+    (ffi_from_observation obs1)
+    (ffi_from_observation obs2)`,
+  rw[ffi_state_rel_def,ffi_from_observation_def,
+     ffiTheory.initial_ffi_state_def]
+  \\ rw[botworld_serialiseTheory.botworld_initial_state_def]
+  \\ simp[encoded_ffi_def]
+  \\ simp[botworld_serialiseTheory.encode_observation_def]
+  \\ AP_TERM_TAC \\ AP_TERM_TAC
+  \\ PairCases_on`y` \\ simp[prepare_def]
+  \\ simp[botworld_serialiseTheory.observationsexp_def]
+  \\ simp[botworld_serialiseTheory.eventsexp_def]
+  \\ AP_TERM_TAC
+  \\ simp[MAP_MAP_o,MAP_EQ_f,FORALL_PROD,if_focal_def]
+  \\ rw[]
+  \\ simp[botworld_serialiseTheory.robotsexp_def]);
+
+val evaluate_botworld_prog_ffi =
+  MATCH_MP evaluate_prog_ffi_extensional botworld_call_FFI_invariant
+
+val preamble_env_ffi = Q.store_thm("preamble_env_ffi",
+  `preamble_env (ffi_from_observation obs) = (st,env) ⇒
+    st.ffi = (ffi_from_observation obs)`,
+  cheat);
+
+val preamble_env_ignores_ffi = Q.store_thm("preamble_env_ignores_ffi",
+  `preamble_env ffi1 = (st,env1) ∧
+   preamble_env ffi2 = (st',env2)
+   ⇒
+   st' = st with ffi := st'.ffi ∧ env1 = env2`,
+  cheat);
+
+val print_sexp_11 = Q.store_thm("print_sexp_11[simp]",
+  `print_sexp x = print_sexp y ⇔ x = y`,
+  cheat);
+
+val outputsexp_11 = Q.store_thm("outputsexp_11[simp]",
+  `outputsexp x = outputsexp y ⇔ x = y`,
+  Cases_on`x` \\ Cases_on`y`
+  \\ simp[botworld_serialiseTheory.outputsexp_def]
+  \\ cheat);
+
+val encode_output_inj = Q.store_thm("encode_output_inj",
+  `encode_output x = encode_output y ⇒ x = y`,
+  rw[botworld_serialiseTheory.encode_output_def]
+  \\ (holSyntaxLibTheory.MAP_EQ_MAP_IMP
+      |> ONCE_REWRITE_RULE[IMP_ANTISYM_RULE SWAP_IMP (Q.SPECL[`P`,`Q`](Q.GENL[`P`,`Q`]SWAP_IMP))]
+      |> drule)
+  \\ impl_tac
+  >- ( simp[] \\ metis_tac[ORD_11,LESS_MOD,ORD_BOUND] )
+  \\ simp[]);
+
+val run_policy_ffi_with_memory = Q.store_thm("run_policy_ffi_with_memory",
+  `x' = x with robotActions updated_by (MAP (if_focal nm' (with_memory p' ## I))) ⇒
+   run_policy p ck (nm,x',private a) = run_policy p ck (nm,x,private a)`,
+  fs[run_policy_def]
+  \\ rpt(pairarg_tac \\ fs[])
+  \\ imp_res_tac preamble_env_ffi
+  \\ match_tac([mg.a"1"`_`,mg.a"2"`_`],fn(a,t)=>
+       preamble_env_ignores_ffi
+       |> REWRITE_RULE[GSYM AND_IMP_INTRO]
+       |> GEN_ALL
+       |> INST_TYPE[beta|->``:botworld_ffi_state``]
+       |> drule_thm(a"1")
+       \\ disch_then(drule_thm(a"2")))
+  \\ rw[] \\ fs[]
+  \\ match_tac([mg.a"1"`_`,mg.a"2"`_`],fn(a,t)=>
+       evaluate_botworld_prog_ffi
+       |> ONCE_REWRITE_RULE[CONJ_COMM]
+       |> REWRITE_RULE[GSYM AND_IMP_INTRO]
+       |> GEN_ALL
+       |> drule_thm (a"1")
+       \\ disch_then (drule_thm(a"2")))
+  \\ simp[ffi_rel_def]
+  \\ impl_tac
+  >- (
+    match_mp_tac (GEN_ALL ffi_from_observation_with_memory)
+    \\ simp[prepare_def,EXISTS_PROD]
+    \\ metis_tac[])
+  \\ simp[ffi_state_rel_def]
+  \\ rw[encoded_ffi_def]
+  \\ imp_res_tac encode_output_inj \\ fs[]);
+
+val runMachine_ffi_with_memory = Q.store_thm("runMachine_ffi_with_memory",
+  `x' = x with robotActions updated_by (MAP (if_focal nm (with_memory p ## I))) ⇒
+   runMachine (prepare x' y) = runMachine (prepare x y)`,
+  strip_tac \\ imp_res_tac run_policy_ffi_with_memory
+  \\ PairCases_on`y` >> rw[runMachine_def,prepare_def]);
+
 val updateInventory_const = Q.store_thm("updateInventory_const[simp]",
   `(SND(updateInventory sq nm ra)).memory = (FST ra).memory ∧
    (SND(updateInventory sq nm ra)).frame = (FST ra).frame ∧
@@ -1409,9 +1743,11 @@ val steph_fill_step = Q.store_thm("steph_fill_step",
     \\ reverse IF_CASES_TAC \\ fs[]
     >- (
       qmatch_goalsub_abbrev_tac`prepare x'`
-      \\ cheat
-      (* need to show that information hiding means changing the memory of
-         robot in an event doesn't affect run_policy *))
+      \\ ONCE_REWRITE_TAC[GSYM PAIR]
+      \\ simp[] \\ AP_TERM_TAC
+      \\ match_mp_tac (GEN_ALL runMachine_ffi_with_memory)
+      \\ simp[Abbr`x'`,event_component_equality,MAP_EQ_f,FORALL_PROD,if_focal_def]
+      \\ metis_tac[] )
     \\ simp[prepare_def,runMachine_def,UNCURRY,robot_component_equality]
     \\ drule (GEN_ALL same_name_same_action) \\ simp[]
     \\ disch_then drule
@@ -1449,7 +1785,11 @@ val steph_fill_step = Q.store_thm("steph_fill_step",
     \\ fs[]
     \\ qmatch_goalsub_abbrev_tac`(_,x',_)`
     \\ `run_policy p r.processor (s.focal_name,x',private a) =
-        run_policy p r.processor (s.focal_name,x,private a)` by cheat (* same info hiding *)
+        run_policy p r.processor (s.focal_name,x,private a)`
+    by (
+      match_mp_tac (GEN_ALL run_policy_ffi_with_memory)
+      \\ simp[Abbr`x'`,event_component_equality,MAP_EQ_f,FORALL_PROD,if_focal_def]
+      \\ metis_tac[])
     \\ rfs[])
   \\ simp[MAP_GENLIST]
   \\ simp[GENLIST_FUN_EQ]
@@ -1466,145 +1806,16 @@ val steph_fill_step = Q.store_thm("steph_fill_step",
   \\ simp[runMachine_def,UNCURRY,robot_component_equality]
   \\ qmatch_goalsub_abbrev_tac`(_,x'',_)`
   \\ qmatch_goalsub_abbrev_tac`(nm,x'',_)`
-  \\ cheat (* same info hiding *));
-
-open terminationTheory
-
-val ffi_state_rel_def = Define`
-  ffi_state_rel R s1 s2 ⇔ R s1.ffi_state s2.ffi_state ∧
-                          s2 = s1 with ffi_state := s2.ffi_state`;
-
-val ffi_rel_def = Define`
-  ffi_rel R s1 s2 ⇔
-    ffi_state_rel R s1.ffi s2.ffi ∧
-    s2 = s1 with ffi := s2.ffi`;
-
-val ffi_rel_dec_clock = Q.store_thm("ffi_rel_dec_clock",
-  `ffi_rel R s1 s2 ⇒
-   ffi_rel R (dec_clock s1) (dec_clock s2)`,
-  EVAL_TAC \\ rw[semanticPrimitivesTheory.state_component_equality]);
-
-val ffi_rel_same_clock = Q.store_thm("ffi_rel_same_clock",
-  `ffi_rel R s1 s2 ⇒ s1.clock = s2.clock`,
-  EVAL_TAC \\ rw[semanticPrimitivesTheory.state_component_equality]);
-
-val ffi_rel_same_refs = Q.store_thm("ffi_rel_same_refs",
-  `ffi_rel R s1 s2 ⇒ s1.refs = s2.refs`,
-  EVAL_TAC \\ rw[semanticPrimitivesTheory.state_component_equality]);
-
-fun extends_tac (tac:tactic) ((g as (asl,w)):goal) =
-  let
-    val asms1 = HOLset.fromList Term.compare asl
-    val (gs,v) = tac g
-    fun extends asl =
-      let
-        val asms2 = HOLset.fromList Term.compare asl
-      in not (HOLset.isEmpty (HOLset.difference(asms2,asms1))) end
-  in
-    (assert(List.all (extends o #1)) gs,v)
-  end
-
-val call_FFI_invariant_def = Define`
-  call_FFI_invariant R ⇔
-  ∀ffi ffi'. R ffi.ffi_state ffi'.ffi_state ⇒
-    ∀i ws.
-      let (ffj,vs) = call_FFI ffi i ws in
-      let (ffj',vs') = call_FFI ffi' i ws in
-        R ffj.ffi_state ffj'.ffi_state
-        ∧ ffj' = ffj with ffi_state := ffj'.ffi_state
-        ∧ vs = vs'`;
-
-val do_app_ffi_extensional = Q.store_thm("do_app_ffi_extensional",
-  `call_FFI_invariant R ∧
-   ffi_state_rel R ffi1 ffi2 ⇒
-   OPTION_REL
-    (λ((refs1,ffi1),res1) ((refs2,ffi2),res2).
-       refs1 = refs2 ∧ res1 = res2 ∧
-       ffi2 = ffi1 with ffi_state := ffi2.ffi_state ∧
-       R ffi1.ffi_state ffi2.ffi_state)
-    (do_app (refs,ffi1) op es)
-    (do_app (refs,ffi2) op es)`,
-  (match1_tac(mg.acb`o_ : 'a option`,(fn(a,t)=>extends_tac(Cases_on`^(t("o"))` \\fs[]\\rveq))))
-  \\ fs[OPTREL_def]
-  \\ rpt (match1_tac(mg.acb`o_ : 'a # 'b`,(fn(a,t)=>extends_tac(Cases_on`^(t("o"))` \\fs[]\\rveq))))
-  >- (
-    reverse(Cases_on`op`)\\fs[semanticPrimitivesTheory.do_app_def]
-    \\ every_case_tac \\ fs[UNCURRY]
-    \\ spose_not_then strip_assume_tac
-    \\ fs[call_FFI_invariant_def,ffi_state_rel_def]
-    \\ first_x_assum drule
-    \\ simp[]
-    \\ qmatch_assum_rename_tac`call_FFI _ i ws = _`
-    \\ map_every qexists_tac[`i`,`ws`]
-    \\ simp[]
-    \\ spose_not_then strip_assume_tac
-    \\ fs[] )
-  \\ rw[ffi_state_rel_def,ffiTheory.ffi_state_component_equality]
-  \\ fs[evalPropsTheory.do_app_cases,semanticPrimitivesTheory.do_app_def] \\ rw[]
-  \\ every_case_tac \\ fs[]
-  \\ spose_not_then strip_assume_tac
-  \\ fs[call_FFI_invariant_def]
-  \\ first_x_assum drule
-  \\ simp[]
-  \\ qmatch_assum_rename_tac`call_FFI _ i ws = _`
-  \\ map_every qexists_tac[`i`,`ws`]
-  \\ simp[]
-  \\ spose_not_then strip_assume_tac
-  \\ fs[]
-  \\ fs[ffiTheory.ffi_state_component_equality]);
-
-val evaluate_ffi_extensional = Q.store_thm("evaluate_ffi_extensional",
-  `call_FFI_invariant R ⇒
-   (∀st env es st' res res' st2 st2'.
-      ffi_rel R st st' ∧
-      evaluate st env es = (st2,res) ∧
-      evaluate st' env es = (st2',res')
-      ⇒ res = res' ∧ ffi_rel R st2 st2') ∧
-   (∀st env v pes err_v st' res res' st2 st2'.
-       ffi_rel R st st' ∧
-       evaluate_match st env v pes err_v = (st2,res) ∧
-       evaluate_match st' env v pes err_v = (st2',res')
-       ⇒ res = res' ∧ ffi_rel R st2 st2')`,
-  strip_tac
-  \\ ho_match_mp_tac evaluate_ind
-  \\ rpt conj_tac
-  \\ rpt gen_tac \\ simp[evaluate_def] \\ strip_tac
-  \\ rveq \\ rpt gen_tac \\ fs[] \\ strip_tac
-  \\ TRY (
-    every_case_tac
-  \\ rpt (qpat_assum`_ ∧ _`strip_assume_tac) \\ rveq
-  \\ fs[] \\ rfs[] \\ rveq
-  \\ imp_res_tac ffi_rel_same_refs \\ fs[]
-  \\ first_x_assum drule \\ fs[]
-  \\ rpt( strip_tac \\ rveq)
-  \\ spose_not_then strip_assume_tac \\ fs[] \\ rveq
-  \\ first_x_assum drule \\ fs[])
-  (* App case *)
-  \\ every_case_tac
-  \\ rpt (qpat_assum`_ ∧ _`strip_assume_tac) \\ rveq
-  \\ fs[] \\ rfs[] \\ rveq
-  \\ imp_res_tac ffi_rel_same_refs \\ fs[]
-  \\ first_x_assum drule \\ fs[]
-  \\ rpt( strip_tac \\ rveq)
-  \\ spose_not_then strip_assume_tac \\ fs[] \\ rveq
-  \\ imp_res_tac ffi_rel_dec_clock
-  \\ imp_res_tac ffi_rel_same_clock \\ fs[]
-  \\ TRY(first_x_assum drule \\ fs[])
-  \\ imp_res_tac ffi_rel_same_refs \\ fs[]
-  \\ imp_res_tac do_app_ffi_extensional
-  \\ fs[ffi_rel_def,
-        semanticPrimitivesTheory.state_component_equality,
-        funBigStepTheory.dec_clock_def]
-  \\ match_tac(
-       [mg.a"h"`ffi_state_rel R ffi_ _`,
-        mg.bau`do_app (refs_,ffi_) op_ es_`
-       ],
-       fn(a,t)=>first_x_assum(drule_thm(a"h")) \\ simp[]
-                \\ map_every (exists_tac o t) ["refs","op","es"])
-  \\ simp[OPTREL_def]
-  \\ spose_not_then strip_assume_tac \\ fs[]
-  \\ rveq \\ fs[]
-  \\ fs[ffi_state_rel_def]);
+  \\ match1_tac(mg.bc`p_:'a # 'b`,fn (a,t) => Cases_on`^(t"p")`) \\ fs[]
+  \\ match1_tac(mg.bc`p_:'a # 'b`,fn (a,t) => Cases_on`^(t"p")`) \\ fs[]
+  \\ ONCE_REWRITE_TAC[CONJ_COMM]
+  \\ REWRITE_TAC[GSYM PAIR_EQ]
+  \\ pop_assum (SUBST_ALL_TAC o SYM)
+  \\ pop_assum (SUBST_ALL_TAC o SYM)
+  \\ match_mp_tac (GEN_ALL run_policy_ffi_with_memory)
+  \\ unabbrev_all_tac \\ simp[event_component_equality]
+  \\ simp[MAP_MAP_o,MAP_EQ_f,FORALL_PROD,if_focal_def]
+  \\ metis_tac[]);
 
 (*
 val LENGTH_localActions = Q.store_thm("LENGTH_localActions[simp]",
